#+latex_class: sandy-article
#+latex_compiler: xelatex
#+options: ':nil *:t -:t ::t <:t H:3 \n:nil ^:t arch:headline author:t
#+options: broken-links:nil c:nil creator:nil d:(not "LOGBOOK") date:t e:t
#+options: email:t f:t inline:t num:t p:nil pri:nil prop:nil stat:t tags:t
#+options: tasks:t tex:t timestamp:t title:t toc:nil todo:t |:t num:nil
#+html_head: <link rel="stylesheet" href="https://sandyuraz.com/styles/org.min.css">
#+language: en

#+title: Homework 2 Oracle
#+subtitle: MATH 220 Spring 2021
#+author: Sandy Urazayev
#+date: 52; 12021 H.E.
#+email: University of Kansas (ctu@ku.edu)

Go back to the [[../../][home page]]

[[./index.pdf][[View the PDF version]â€‹]]

* Chapter 2.1
** Problem 13
   #+attr_html: :width 80%
   [[./13.png]]
*** Part a
    As $t$ gets infinitely large, it simply oscillates in an inverse cosine
    fashion. $a$ does give the function an initial starting point, to which it
    starts oscillating from. That would probably be $a + \pi$ because
    $2cos(t)$ changes its behaviour every $\pi$ revolution.
*** Part b
    This is a first-order linear differential equation
    of the form $y' + p(t) y = q(t)$. Find
    $\mu(t) = e^{\int{-\frac{1}{2}}}$ and then solve $\frac{d}{dt}(\mu(t)y) = q(t) \mu(t)$
    $\implies y = \frac{\int q(t) \mu(t) dt}{\mu(t)}$. You should get
    \begin{equation*}
            y(t) = ce^{t/2}+\frac{8}{5}\sin(t)-\frac{4}{5}\cos(t)
    \end{equation*}
    Then solving for $y(0)$ and $c$, we have the full solution to be
    \begin{equation*}
            y(t) = (a+\frac{4}{5}e^{t/2})+\frac{8}{5}\sin(t)-\frac{4}{5}\cos(t)
    \end{equation*}
*** Part c
    $y$ oscillates for $a=a_0$
** Problem 15 [FOR GRADE]
*** Part a
    This is again, a first-order linear differential equation, so we do our
    $\mu$ and integration from both sides trick. Recognize that we have to
    divide everything by $t$, so that our lead $y'$ doesn't have a coefficient
    and the method for solving this type of equations is applicable.
    \begin{equation*}
            ty'+(t+1)y = 2 t e^{-t} \iff y' + (\frac{t+1}{t})y = 2 e^{-t}
    \end{equation*}
    After cleaning it up, the actual solution process becomes more or less
    trivial, $\mu(t) = e^{\int{\frac{t+1}{t}}} = te^t$. Then we find for $t>0$
    \begin{equation*}
            y(t) = \frac{ce^{-t}}{t} + e^{-t}t
    \end{equation*}
    Applying $y(1) = a$, then we get
    \begin{equation*}
            y(t) = te^{-t} + \frac{(ea-1)e^{-t}}{t}
    \end{equation*}
    We need $ea-1$ to be equal to zero, then $a_0 = \frac{1}{e}$
*** Part c
    As $t \to 0$, then $y \to 0$. 
** Problem 17 [FOR GRADE]
   Recall the solution to Problem 13. We need to swap the sign on $p(t)$ and
   update the initial value constant solution. We will get
   \begin{equation*}
           y(t) = -\frac{9}{5}e^{t/2}+\frac{8}{5}\sin(t)+\frac{4}{5}\cos(t)
   \end{equation*}
   Set the derivative of $y$ to $0$ and solve for $t$.
   \begin{equation*}
     0 = -\frac{9}{5}\times (-\frac{1}{2}) \times e^{t/2}+\frac{8}{5}\cos(t)-\frac{4}{5}\sin(t)
   \end{equation*}
   You can check the nature of the point by taking $y''$. Finally, we find that
   the local maximum is at $(t, y) = (1.36, 0.82)$. Better approximated values
   are accepted.
** Problem 20
   The solution process is similar to the problem of 17, you should get a
   general solution for $y$:
   \begin{equation*}
           y = -1 - \frac{3}{2}(\sin t + \cos t) + C e^t
   \end{equation*}
   where $C$ is a constant. Solving $y(0) = y_0$ for $y_0$ yields that
   $C = y_0 + \frac{5}{2}$ so then the solution is $y_0 = -\frac{5}{2}$.
** Problem 28
*** Part a
    Recall the form $y' + p(t) y = g(t)$ and solution form of 
    \begin{equation*}
            \frac{d}{dt}(\mu(t)y) = g(t) \mu(t)
    \end{equation*}
    Then if $g(t)=0$, solution
    is $y = A e^{-\int{p(t)dt}}$
*** Part b
    Simply substitute (50) into (48), perform some trivial Chain Rule and
    confirm that
    \begin{equation*}
            A'(t) = g(t) \exp\left(\int p(t) dt\right)
    \end{equation*}
*** Part c
    Substitution is mechanical. Prove that variation of parameters works.
* Chapter 2.2
** Problem 1
   \begin{equation*}
           \frac{dy}{dx} = \frac{x^2}{y}
   \end{equation*}
   then
   \begin{equation*}
           \int y dy = \int x^2 dx
   \end{equation*}
   So the solution is
   \begin{equation*}
           3y^2-2x^3=C
   \end{equation*}
   It's OK to leave the solution implicitly here, otherwise, the explicit
   solution for $y$ can be very nasty.
** Problem 7
   \begin{equation*}
     \frac{dy}{dx} = \frac{y}{x}
   \end{equation*}
   then
   \begin{equation*}
           \int \frac{dy}{y} = \int \frac{dx}{x}
   \end{equation*}
   Then
      \begin{equation*}
              \ln(y) = ln(x) + ln(C) = ln(C\times x)
      \end{equation*}
      $C$ is any constant, then $\ln(C)$ is also a constant.
      Finally, $y = Cx$
** Problem 8 [FOR GRADE]
   \begin{equation*}
           \frac{dy}{dx} = \frac{-x}{y}
   \end{equation*}
   then
   \begin{equation*}
           \int y dy = - \int x dx
   \end{equation*}
   Therefore
   \begin{equation*}
           y^2 + x^2 = C
   \end{equation*}
   It's fine if you wrote $y = \pm \sqrt{C - x^2}$
** Problem 21
   \begin{equation*}
           y' = \frac{ty(4-y)}{3}, \quad y(0) = y_0
   \end{equation*}
*** Part a
    As $t \to \infty$, then $y \to 4$
*** Part b
    First, you will have to solve the system, which is a first-order separable
    ordinary differential equation.  The implicit solution is
    \begin{equation*}
            \frac{3}{4} \ln(\frac{4}{4-5}) = \frac{t^2}{2} + C
    \end{equation*}
    where $C = \frac{3}{4} \ln(\frac{y_0}{4-y_0})$.

    Solve for $t$, so
    \begin{equation*}
      t = \sqrt{\frac{3}{2} \ln\left(\frac{y(4-y_0)}{y_0(4-y)}\right)}
    \end{equation*}
    Use $y = 3.98$ and $y_0 = 0.5$, then $t \approx 3.29527$.
** Problem 25
*** Part a
    Simple divide both the numerator and the denominator by $x$.
*** Part b
    You should get
    \begin{equation*}
            \frac{dy}{dx} = v + x \frac{dv}{dx}
    \end{equation*}
*** Part c
    This is simply to show.
*** Part d
    Yet another separable equation, you should get the implicit solution
        \begin{equation*}
          x^4 \left| 2 - v \right| \left| v + 2 \right|^3 = C
        \end{equation*}
*** Part e
    Rearrange to get
    \begin{equation*}
            |y+2x|^3 |2x-y| = C
    \end{equation*}
*** Part f
    It's like a 1/x star. 
