#+latex_class: sandy-article
#+latex_compiler: xelatex
#+options: ':nil *:t -:t ::t <:t H:3 \n:nil ^:t arch:headline author:t
#+options: broken-links:nil c:nil creator:nil d:(not "LOGBOOK") date:t e:t
#+options: email:t f:t inline:t num:t p:nil pri:nil prop:nil stat:t tags:t
#+options: tasks:t tex:t timestamp:t title:t toc:nil todo:t |:t num:nil
#+html_head: <link rel="stylesheet" href="https://sandyuraz.com/styles/org.min.css">
#+language: en

#+title: Homework 5 Oracle
#+subtitle: MATH 220 Spring 2021
#+author: Sandy Urazayev
#+date: 93; 12021 H.E.
#+email: University of Kansas (ctu@ku.edu)

[[./index.pdf][[View the PDF version]â€‹]]

* Section 3.1
** Problem 9
   \begin{equation*}
     y'' + 3y' = 0, \quad y(0) = -2, \quad y'(0) = 3
   \end{equation*}
   Since this is a linear homogeneous constant-coefficient ODE, the solution is
   of the form $y = e^{rt}$
   \begin{equation*}
     y=e^{rt} \quad \implies \quad y' = re^{rt} \quad \implies \quad y'' = r^2 e^{rt}
   \end{equation*}
   Substitute those expressions into the ODE
   \begin{equation*}
     r^2 e^{rt} + 3(re^{rt}) = 0
   \end{equation*}
   Divide both sides by $e^{rt}$
   \begin{equation*}
     r^2 + 3r = 0
   \end{equation*}
   Roots of this polynomial are $r_0 = -3$ and $r_1 = 0$. Two solutions to the
   ODE are $y=e^{-3t}$ and $y=e^0=1$. Therefore, the general solution is
   \begin{equation*}
     y(t) = C_1 e^{-3t} + C_2
   \end{equation*}
   Differentiating $y$ gives us
   \begin{equation*}
     y'(t) = -3C_1 e^{-3t}
   \end{equation*}
   Now, we can determine our constants by applying the two initial conditions we
   know
   \begin{equation*}
     \begin{cases}
       y(0) = C_1 + C_2 = -2\\
       y'(0) = -3C_1 = 3
     \end{cases}
   \end{equation*}
   Therefore $C_1 = -1$ and $C_2 = -1$, therefore
   \begin{equation*}
     y(t) = -e^{-3t} - 1
   \end{equation*}
   This solution converges to $-1$ as $t \to \infty$.
** Problem 13 [FOR GRADE]
   Find a differential equation whose general solution is
   \begin{equation*}
     y=c_{1} e^{2 t}+c_{2} e^{-3 t}
   \end{equation*}
   We see the roots are $r_0 = -3$ and $r_1 = 2$. Alternatively, you can make a
   set of solutions, and call it $r = \{-3,2\}$. So
   \begin{align*}
     (r+3)(r-2)&=0 \\
     \implies r^2 + r - 6 &= 0
   \end{align*}
   Multiply both sides by $e^{rt}$
   \begin{align*}
     r^2e^{rt} + re^{rt} - 6e^{rt} = 0
   \end{align*}
   Therefore, the differential equation is
   \begin{align*}
     y'' + y' - 6y = 0
   \end{align*}
** Problem 16
   This is a linear homogeneous constant-coefficient ODE, apply the same method
   as in Problem 9. Find that $r = \{-1, 2\}$ and the general solution is
   \begin{align*}
     y(t) = C_1 e^{-t} + C_2 e^{2t}
   \end{align*}
   The derivative would be
   \begin{align*}
     y'(t) = -C_1 e^{-t} + 2 C_2 e^{2t}
   \end{align*}
   Let us solve the initial conditions
      \begin{align*}
        \begin{cases}
          y(0) = C_1 + C_2 = \alpha\\
          y'(0) = -C_1 + 2C_2 = 2
        \end{cases}
        \implies \begin{cases}
          C_1 = \frac{2}{3}(\alpha -1)\\
          C_2 = \frac{1}{3}(\alpha +2)
        \end{cases}
      \end{align*}
      Therefore,
      \begin{align*}
        y(t) = \frac{2}{3}(\alpha -1)e^{-t} + \frac{1}{3}(\alpha +2)e^{2t}
      \end{align*}
      We can see that if $t \to \infty$, then $y \to \infty$. Therefore, set
      $\alpha = -2$.
** Problem 19
   \begin{align*}
     y'' + 5y' + 6y = 9, \quad y(0) = 2, \quad y'(0) = \beta,
   \end{align*}
   where $\beta > 0$.
*** Part (a)
    This is a linear homogeneous constant-coefficient ODE, find that
    $r = {-\frac{1}{2}, \frac{1}{2}}$. The two solutions are
    \begin{align*}
      y(t) = C_1 e^{-\frac{t}{2}} + C_2 e^{\frac{t}{2}}
    \end{align*}
    Then
    \begin{align*}
      y'(t) = -\frac{C_1}{2} e^{-\frac{t}{2}} + \frac{C_2}{2} e^{\frac{t}{2}}
    \end{align*}
    Solve
    \begin{align*}
      \begin{cases}
        y(0) = C_1 + C_2 = 2\\
        y'(0) = -\frac{C_1}{2} + \frac{C_2}{2} = \beta
      \end{cases} \implies
      \begin{cases}
        C_1 = 1 - \beta\\
        C_2 = 1 + \beta
      \end{cases}
    \end{align*}
    Finally,
    \begin{align*}
      y(t) = (1 - \beta)e^{-\frac{t}{2}} + (1+\beta)e^{\frac{t}{2}}
    \end{align*}
    To prevent the solution from going to the infinity and beyond, set
    $\beta=-1$.
*** Part (b, c, d)
    See Professor Van Vleck's notes on this problem.
** Problem 21 [FOR GRADE]
   \begin{align*}
     ay'' + by' + cy = 0,
   \end{align*}
   where $a, b, c \in \mathbb{R}$ and $a > 0$.

   This is yet again another linear homogeneous constant-coefficient ODE. Find
   that
  \begin{align*}
a\left(r^{2} e^{r t}\right)+b\left(r e^{r t}\right)+c\left(e^{r t}\right)=0
\end{align*}
Divide both sides by $e^{r t}$
\begin{align*}
a r^{2}+b r+c=0 \\
\implies r=\frac{-b \pm \sqrt{b^{2}-4 a c}}{2 a}
\end{align*}
*** Part (a)
    For the roots to be real, different and negative, $b^2 - 4ac > 0$ and $b>0$
    and $c>0$.
*** Part (b)
    For the roots to be real with opposite signs, $b^2 - 4ac > 0$, $b = 0$.
*** Part (c)
    For the roots to be real, different and positive, $b^2-4ac>0$ and $b<0$.
*** Note:
    Here are the book's answers, which are also accepted
    a. $b>0$ and $0<c<b^2/(4a)$
    b. $c<0$
    c. $b<0$ and $0<c<b^2/(4a)$
* Section 3.2
** Problem 5
   The Wronskian of these two functions is
\begin{align*}
W &=\left|\begin{array}{cc}
\cos ^{2} \theta & 1+\cos 2 \theta \\
\frac{d}{d \theta}\left(\cos ^{2} \theta\right) & \frac{d}{d \theta}(1+\cos 2 \theta)
\end{array}\right| \\
&=\left|\begin{array}{cc}
\cos ^{2} \theta & 1+\cos 2 \theta \\
2 \cos \theta(-\sin \theta) & -2 \sin 2 \theta
\end{array}\right| \\
&=\cos ^{2} \theta(-2 \sin 2 \theta)-(1+\cos 2 \theta)[2 \cos \theta(-\sin \theta)] \\
&=-2 \cos ^{2} \theta \sin 2 \theta+2 \sin \theta \cos \theta(1+\cos 2 \theta) \\
&=-2 \cos ^{2} \theta(2 \sin \theta \cos \theta)+2 \sin \theta \cos \theta\left(1+2 \cos ^{2} \theta-1\right) \\
&=-4 \cos ^{2} \theta \sin \theta \cos \theta+4 \sin \theta \cos \theta \cos ^{2} \theta \\
&=0
\end{align*}

** Problem 22 [FOR GRADE]
   \begin{align*}
     y'' - y' - 2y = 0
   \end{align*}

   *Note:* Solutions for this problem are based on Jock's solutions.
   
*** Part (a)
    Calculate $W\left(y_{1}, y_{2}\right)$ the Wronskian of $y_{1}$ and
    $y_{2}$.

\begin{align*}
W\left(y_{1}, y_{2}\right) &=\left|\begin{array}{ll}
y_{1} & y_{2} \\
y_{1}^{\prime} & y_{2}^{\prime}
\end{array}\right| \\
&=\left|\begin{array}{cc}
e^{-t} & e^{2 t} \\
-e^{-t} & 2 e^{2 t}
\end{array}\right| \\
&=e^{-t}\left(2 e^{2 t}\right)-e^{2 t}\left(-e^{-t}\right) \\
&=2 e^{t}+e^{t} \\
&=3 e^{t}
\end{align*}

Since $W\left(y_{1}, y_{2}\right) \neq 0, y_{1}$ and $y_{2}$ form a fundamental
set of solutions.

*** Part (b)

    Check that $y_{3}$ is a solution of the ODE.
    
\begin{array}{c}
y_{3}^{\prime \prime}-y_{3}^{\prime}-2 y_{3} \stackrel{?}{=} 0 \\
\frac{d^{2}}{d t^{2}}\left(-2 e^{2 t}\right)-\frac{d}{d t}\left(-2 e^{2 t}\right)-2\left(-2 e^{2 t}\right) \stackrel{?}{=} 0 \\
\left(-8 e^{2 t}\right)-\left(-4 e^{2 t}\right)-2\left(-2 e^{2 t}\right) \stackrel{?}{=} 0 \\
-8 e^{2 t}+4 e^{2 t}+4 e^{2 t} \stackrel{?}{=} 0 \\
0=0
\end{array}

Now check that $y_{4}=e^{-t}+2 e^{2 t}$ is a solution of the ODE.

\begin{array}{c}
y_{4}^{\prime \prime}-y_{4}^{\prime}-2 y_{4} \stackrel{?}{=} 0 \\
\frac{d^{2}}{d t^{2}}\left(e^{-t}+2 e^{2 t}\right)-\frac{d}{d t}\left(e^{-t}+2 e^{2 t}\right)-2\left(e^{-t}+2 e^{2 t}\right) \stackrel{?}{=} 0 \\
\left(e^{-t}+8 e^{2 t}\right)-\left(-e^{-t}+4 e^{2 t}\right)-2\left(e^{-t}+2 e^{2 t}\right) \stackrel{?}{=} 0 \\
e^{-^{\ell}}+8 e^{2 t}+e^{-}-4 e^{2 t}-2 e^{-}-4 e^{2 t} \stackrel{?}{=} 0 \\
0=0
\end{array}

Now check that $y_{5}=2 y_{1}(t)-2 y_{3}(t)=2 e^{-t}-2\left(-2 e^{2 t}\right)=2
e^{-t}+4 e^{2 t}$ is a solution of the ODE. 

\begin{array}{c}
y_{5}^{\prime \prime}-y_{5}^{\prime}-2 y_{5} \stackrel{?}{=} 0 \\
\frac{d^{2}}{d t^{2}}\left(2 e^{-t}+4 e^{2 t}\right)-\frac{d}{d t}\left(2 e^{-t}+4 e^{2 t}\right)-2\left(2 e^{-t}+4 e^{2 t}\right) \stackrel{?}{=} 0 \\
\left(2 e^{-t}+16 e^{2 t}\right)-\left(-2 e^{-t}+8 e^{2 t}\right)-2\left(2 e^{-t}+4 e^{2 t}\right) \stackrel{?}{=} 0 \\
2 e^{-}+16 e^{2 t}+2 e^{-}-8 e^{2 t}-4 e^{-}-8 e^{2 t} \stackrel{?}{=} 0 \\
0=0
\end{array}

*** Part (c)

    Calculate $W\left(y_{1}, y_{3}\right)$, the Wronskian of $y_{1}$ and $y_{3}$.

\begin{aligned}
W\left(y_{1}, y_{3}\right) &=\left|\begin{array}{ll}
y_{1} & y_{3} \\
y_{1}^{\prime} & y_{3}^{\prime}
\end{array}\right| \\
&=\left|\begin{array}{cc}
e^{-t} & -2 e^{2 t} \\
-e^{-t} & -4 e^{2 t}
\end{array}\right| \\
&=e^{-t}\left(-4 e^{2 t}\right)-\left(-2 e^{2 t}\right)\left(-e^{-t}\right) \\
&=-4 e^{t}-2 e^{t} \\
&=-6 e^{t}
\end{aligned}

Since $W\left(y_{1}, y_{3}\right) \neq 0, y_{1}$ and $y_{3}$ form a fundamental set of solutions.

Now calculate $W\left(y_{2}, y_{3}\right)$, the Wronskian of $y_{2}$ and $y_{3}$

\begin{aligned}
W\left(y_{2}, y_{3}\right) &=\left|\begin{array}{ll}
y_{2} & y_{3} \\
y_{2}^{\prime} & y_{3}^{\prime}
\end{array}\right| \\
&=\left|\begin{array}{cc}
e^{2 t} & -2 e^{2 t} \\
2 e^{2 t} & -4 e^{2 t}
\end{array}\right| \\
&=e^{2 t}\left(-4 e^{2 t}\right)-\left(-2 e^{2 t}\right)\left(2 e^{2 t}\right) \\
&=-4 e^{4 t}+4 e^{4 t} \\
&=0
\end{aligned}

Since $W\left(y_{2}, y_{3}\right)=0, y_{2}$ and $y_{3}$ do not form a
fundamental set of solutions. Now calculate $W\left(y_{1}, y_{4}\right)$, the
Wronskian of $y_{1}$ and $y_{4}$ 

\begin{aligned}
W\left(y_{1}, y_{4}\right) &=\left|\begin{array}{ll}
y_{1} & y_{4} \\
y_{1}^{\prime} & y_{4}^{\prime}
\end{array}\right| \\
&=\left|\begin{array}{cc}
e^{-t} & e^{-t}+2 e^{2 t} \\
-e^{-t} & -e^{-t}+4 e^{2 t}
\end{array}\right| \\
&=e^{-t}\left(-e^{-t}+4 e^{2 t}\right)-\left(e^{-t}+2 e^{2 t}\right)\left(-e^{-t}\right) \\
&=-e^{-2 t}+4 e^{t}+e^{-2 t}+2 e^{t} \\
&=6 e^{t}
\end{aligned}

Since $W\left(y_{1}, y_{4}\right) \neq 0, y_{1}$ and $y_{4}$ form a fundamental
set of solutions. Now calculate $W\left(y_{4}, y_{5}\right)$, the Wronskian of
$y_{4}$ and $y_{5}$. 

\begin{aligned}
W\left(y_{4}, y_{5}\right) &=\left|\begin{array}{ll}
y_{4} & y_{5} \\
y_{4}^{\prime} & y_{5}^{\prime}
\end{array}\right| \\
&=\left|\begin{array}{cc}
e^{-t}+2 e^{2 t} & 2 e^{-t}+4 e^{2 t} \\
-e^{-t}+4 e^{2 t} & -2 e^{-t}+8 e^{2 t}
\end{array}\right| \\
&=\left(e^{-t}+2 e^{2 t}\right)\left(-2 e^{-t}+8 e^{2 t}\right)-\left(2 e^{-t}+4 e^{2 t}\right)\left(-e^{-t}+4 e^{2 t}\right) \\
&=-2 e^{-2 t}+8 e^{t}-4 e^{t}+16 e^{4 t}-\left(-2 e^{-2 t}+8 e^{t}-4 e^{t}+16 e^{4 t}\right) \\
&=0
\end{aligned}

Since $W\left(y_{4}, y_{5}\right)=0, y_{4}$ and $y_{5}$ do not form a fundamental set of solutions.
** Problem 24
   \begin{align*}
     (\cos t)y'' +(\sin t)y' -ty = 0
   \end{align*}
   Then
   \begin{align*}
     y'' + \frac{\sin t}{\cos t} - \frac{t}{\cos t}y = 0
   \end{align*}
   so
   \begin{align*}
     p(t) = \tan t
   \end{align*}
   Then
   \begin{align*}
     W = C \exp\left(-\int \tan t dt \right)
   \end{align*}
   By Abel's Theorem
   \begin{align*}
     W = C \exp \left( \ln (cos t) \right) \implies W = C\times \cos t
   \end{align*}
** Problem 31
   The equation
   \begin{align*}
           P(x) y^{\prime \prime}+Q(x) y^{\prime}+R(x) y=0
   \end{align*}
   is said to be exact if it can be written in the form
\begin{align*}
	\left(P(x) y^{\prime}\right)^{\prime}+(f(x) y)^{\prime}=0
\end{align*}
where $f(x)$ is to be determined in terms of $P(x), Q(x),$ and $R(x)$ The latter equation can be integrated once immediately, resulting in a first-order linear equation for $y$ that can be solved as in Section 2.1. By equating the coefficients of the preceding equations and then eliminating $f(x)$, show that a necessary condition for exactness is
\begin{align*}
	P^{\prime \prime}(x)-Q^{\prime}(x)+R(x)=0
\end{align*}
It can be shown that this is also a sufficient condition.
