#+latex_class: sandy-article
#+latex_compiler: xelatex
#+options: ':nil *:t -:t ::t <:t H:3 \n:nil ^:t arch:headline author:t
#+options: broken-links:nil c:nil creator:nil d:(not "LOGBOOK") date:t e:t
#+options: email:t f:t inline:t num:t p:nil pri:nil prop:nil stat:t tags:t
#+options: tasks:t tex:t timestamp:t title:t toc:nil todo:t |:t num:nil

#+language: en

#+title: Homework 6 Oracle
#+subtitle: MATH 220 Spring 2021
#+author: Sandy Urazayev
#+date: 93; 12021 H.E.
#+email: University of Kansas (ctu@ku.edu)

* Homework 6 Oracle

Go back to the [[../../][home page]]

[[./index.pdf][View the PDF versionâ€‹]]

** Section 3.3
*** Problem 7
   \begin{align*}
     y'' + 2y' + 2y = 0
   \end{align*}
   Find that $r = \{-1 - i, -1 + i\}$. Then
   \begin{align*}
     y(t) = C_1 e^{-t} \cos (t) + C_2 e^{-t} \sin (t)
   \end{align*}
*** Problem 13 [FOR GRADE]
   \begin{align*}
     y'' - 2y' + 5y = 0, \quad y(\pi/2) = 0, \quad y'(\pi / 2) = 2
   \end{align*}
   Find that $r = \{1+2i,1-2i\}$. Then
   \begin{align*}
     y(t) = C_1 e^t \cos (2t) + C_2 e^t \sin (2t)
   \end{align*}
   Let us apply the initial conditions
   \begin{align*}
     \begin{cases}
       y(\pi/2)=0\\
       y'(\pi/2)=2
       \end{cases} \implies
     \begin{cases}
       C_1 = 0\\
       C_2 = -\frac{1}{e^{\pi/2}}
       \end{cases}
   \end{align*}
   Finally,
   \begin{align*}
     y(t) = -\frac{1}{e^{\pi/2}} e^t \sin (2t)
   \end{align*}
*** Problem 17
   \begin{align*}
     5u'' + 2u' + 7u = 0, \quad u(0) = 2, \quad u'(0) = 1
   \end{align*}
**** Part (a)
    Find that
    $r = \{-\frac{1}{5} - i\frac{\sqrt{34}}{5}, -\frac{1}{5} +
    i\frac{\sqrt{34}}{5}\}$. Then
    \begin{align*}
      \begin{cases}
        u(0) = 2\\
        u'(0) = 1
      \end{cases} \implies
      \begin{cases}
        C_1 = 2\\
        C_2 = \frac{7}{\sqrt{34}}
      \end{cases}
    \end{align*}
    Finally,
    \begin{align*}
      u(t) = 2 e^{-t/5} \cos\left(\frac{\sqrt{34}t}{5}\right) + \frac{7}{\sqrt{34}} e^{-t/5} \sin\left(\frac{\sqrt{34}t}{5}\right)
    \end{align*}
**** Part (b)
    \begin{align*}
      T \approx 14.512
    \end{align*}
*** Problem 19
      \begin{aligned} W\left(e^{\lambda t} \cos \mu t, e^{\lambda t} \sin \mu
              t\right) & =\left|\begin{array}{cc}e^{\lambda t} \cos \mu t & e^{\lambda t}
                      \sin \mu t                                   \\ \frac{d}{d t}\left(e^{\lambda t} \cos \mu t\right) & \frac{d}{d
                              t}\left(e^{\lambda t} \sin \mu t\right)\end{array}\right|
              \\ &=\left|\begin{array}{cc}e^{\lambda t} \cos \mu t & e^{\lambda t} \sin \mu
                      t                                                     \\ \lambda e^{\lambda t} \cos \mu t-\mu e^{\lambda t} \sin \mu t \quad
                      \lambda e^{\lambda t} \sin \mu t+\mu e^{\lambda t} \cos \mu
                      t\end{array}\right| \\ &=e^{\lambda t} \cos \mu t\left(\lambda e^{\lambda t}
              \sin \mu t+\mu e^{\lambda t} \cos \mu t\right)-e^{\lambda t} \sin \mu
              t\left(\lambda e^{\lambda t} \cos \mu t-\mu e^{\lambda t} \sin \mu t\right)
              \\ &=\lambda e^{2 \lambda t} \cos \mu t \sin \mu t+\mu e^{2
                              \lambda t} \cos ^{2} \mu t\lambda e^{2 \lambda t} \cos \mu t
              \sin \mu t+\mu e^{2 \lambda t} \sin ^{2} \mu t     \\ &=\mu e^{2 \lambda
              t}\left(\cos ^{2} \mu t+\sin ^{2} \mu t\right)     \\ &=\mu e^{2 \lambda t}
      \end{aligned}
   
** Section 3.4
*** Problem 1
   \begin{align*}
     y'' - 2y' + y = 0
   \end{align*}
   Then
   \begin{align*}
     r^2 - 2r + 1 = 0
   \end{align*}
   So $r = 1$, finally
   \begin{align*}
     y(t) = C_1 e^t + C_2 t e^t
   \end{align*}
*** Problem 8 [FOR GRADE]
   \begin{align*}
     2y'' + 2y' + y = 0
   \end{align*}
   Then
   \begin{align*}
     2r^2 + 2r + 1 = 0
   \end{align*}
   So $r = \{-1/2 - 1/2i, -1/2 + 1/2i\}$. Finally,
   \begin{align*}
     y(t) = C_1 e^{-t/2} \cos \left(\frac{1}{2}t\right) + C_2 e^{-t/2} \sin \left(\frac{1}{2}t\right)
   \end{align*}
*** Problem 11
   \begin{align*}
     y'' + 4y' + 4y = 0, \quad y(-1)=2, \quad y'(-1) = 1
   \end{align*}
   Then $r=\{-2\}$. So
   \begin{align*}
     y(t) = C_1 e^{-2t} + C_2 t e^{-2t}
   \end{align*}
   Taking the derivative
   \begin{align*}
     y'(t) = C_1 e^{-2t} - 2 C_1t e^{-2t} - 2 C_2 e^{-2t}
   \end{align*}
   Applying the initial conditions
   \begin{align*}
     \begin{cases}
       y(-1) = -C_1e^2 + C_2 e^2 = 2\\
       y'(-1) = C_1 e^2 + 2 C_1 e^2 - 2 C_2 e^2 = 1
     \end{cases} \implies
     \begin{cases}
       C_1 = \frac{5}{e^2}\\
       C_2 = \frac{7}{e^2}
     \end{cases}
   \end{align*}
   Therefore
   \begin{align*}
     y(t) = \frac{5}{e^2}te^{-2t} + \frac{7}{e^2}e^{-2t}
   \end{align*}
   As $t \to \infty$, $y \to 0$.
*** Problem 18 [FOR GRADE]
   \begin{align*}
     t^2 y'' - 4 t y' + 6 y = 0, \quad t > 0; \quad y_1(t) = t^2
   \end{align*}
   Let us apply the method of reduction
   Let the general solution be of the form
   \begin{align*}
     y(t) = v(t) y_1(t) = t^2v(t)
   \end{align*}
   Let us find the derivatives
   \begin{align*}
     y_2'(t) &= t^2v'(t) + 2tv(t)\\
     y_2''(t) &= t^2v''(t) + 2tv'(t) + 2tv'(t) + 2v(t)
   \end{align*}
   Let us substitute the above into our original ODE
   \begin{align*}
     t^2 (t^2v''(t) + 2tv'(t) + 2tv'(t) + 2v(t)) -4t (t^2v'(t) + 2tv(t)) + 6(t^2v(t)) = 0
   \end{align*}
   Simplifying yields
   \begin{align*}
     t^4 v''(t) + 3t^3v'(t) + t^2v(t) - 4t^3v'(t) -8t^2v(t) + 6t^2v(t) = 0\\
     t^4v''(t) = 0
   \end{align*}
   Then
   \begin{align*}
     v''(t) = 0
   \end{align*}
   Integrate both sides
   \begin{align*}
     v'(t) = C_1\\
     v(t)  = C_1 t + C_2
   \end{align*}
   Finally, the general solution is
   \begin{align*}
     y(t) = (C_1t + C_2)t^2 = C_1t^3 + C_2t^2 = C_1 y_1(t) + C_2 y_2(t)
   \end{align*}
   and the second solution is $y_2(t) = t^3$.
