#+latex_class: sandy-article
#+latex_compiler: xelatex
#+options: ':nil *:t -:t ::t <:t H:3 \n:nil ^:t arch:headline author:t
#+options: broken-links:nil c:nil creator:nil d:(not "LOGBOOK") date:t e:t
#+options: email:t f:t inline:t num:t p:nil pri:nil prop:nil stat:t tags:t
#+options: tasks:t tex:t timestamp:t title:t toc:nil todo:t |:t num:nil
#+html_head: <link rel="stylesheet" href="https://sandyuraz.com/styles/org.min.css">
#+language: en

#+title: Homework 11 Oracle
#+subtitle: MATH 220 Spring 2021
#+author: Sandy Urazayev
#+date: 128; 12021 H.E.
#+email: University of Kansas (ctu@ku.edu)

[[./index.pdf][[View the PDF version]â€‹]]

Solution to these problems are provided by STEM Jock.

* Section 6.2
  
** Problem 3
   
*** Statement
    \begin{equation*}
 F(s)=\frac{2}{s^{2}+3 s-4}
 \end{equation*}

*** Solution
    Factor the denominator.

    \begin{aligned}
F(s) &=\frac{2}{s^{2}+3 s-4} \\
&=\frac{2}{(s+4)(s-1)} \\
&=\frac{2 / 5}{s-1}-\frac{2 / 5}{s+4}
\end{aligned}

Take the inverse Laplace transform now to get $f(t)$.

$$
f(t)=\frac{2}{5} e^{t}-\frac{2}{5} e^{-4 t}
$$

** Problem 11
   
*** Statement
 $$
    y^{\prime \prime}-2 y^{\prime}+4 y=0 ; \quad y(0)=2, \quad y^{\prime}(0)=0
 $$
   
*** Solution
    Because the ODE is linear, the Laplace transform can be applied to solve it. The Laplace transform of a function $y(t)$ is defined here as
$$
Y(s)=\mathcal{L}\{y(t)\}=\int_{0}^{\infty} e^{-s t} y(t) d t
$$
Consequently, the first and second derivatives transform as follows.


\begin{aligned}
\mathcal{L}\left\{\frac{d y}{d t}\right\} &=s Y(s)-y(0) \\
\mathcal{L}\left\{\frac{d^{2} y}{d t^{2}}\right\} &=s^{2} Y(s)-s y(0)-y^{\prime}(0)
\end{aligned}


Apply the Laplace transform to both sides of the ODE.
$$
\mathcal{L}\left\{y^{\prime \prime}-2 y^{\prime}+4 y\right\}=\mathcal{L}\{0\}
$$
Use the fact that the transform is a linear operator.

\begin{array}{c}
\mathcal{L}\left\{y^{\prime \prime}\right\}-2 \mathcal{L}\left\{y^{\prime}\right\}+4 \mathcal{L}\{y\}=0 \\
{\left[s^{2} Y(s)-s y(0)-y^{\prime}(0)\right]-2[s Y(s)-y(0)]+4 Y(s)=0}
\end{array}

Plug in the initial conditions, $y(0)=2$ and $y^{\prime}(0)=0$.

$$
\left[s^{2} Y(s)-2 s\right]-2[s Y(s)-2]+4 Y(s)=0
$$

As a result of applying the Laplace transform, the ODE has reduced to an algebraic equation for
  Solution $Y$ , the transformed solution.

  \begin{equation*}
\begin{array}{c}
s^{2} Y(s)-2 s Y(s)+4 Y(s)-2 s+4=0 \\
\left(s^{2}-2 s+4\right) Y(s)=2 s-4
\end{array}
\end{equation*}

\begin{aligned}
Y(s) &=\frac{2 s-4}{s^{2}-2 s+4} \\
&=\frac{2 s-4}{s^{2}-2 s+1+4-1} \\
&=\frac{2 s-4}{(s-1)^{2}+3} \\
&=\frac{2 s-2-4+2}{(s-1)^{2}+3} \\
&=\frac{2(s-1)-2}{(s-1)^{2}+3} \\
&=2 \frac{s-1}{(s-1)^{2}+3}-\frac{2}{(s-1)^{2}+3} \\
&=2 \frac{s-1}{(s-1)^{2}+3}-\frac{2}{\sqrt{3}} \frac{\sqrt{3}}{(s-1)^{2}+3}
\end{aligned}

Take the inverse Laplace transform of $Y(s)$ now to recover $y(t)$.

\begin{aligned}
y(t) &=\mathcal{L}^{-1}\{Y(s)\} \\
&=\mathcal{L}^{-1}\left\{2 \frac{s-1}{(s-1)^{2}+3}-\frac{2}{\sqrt{3}} \frac{\sqrt{3}}{(s-1)^{2}+3}\right\} \\
&=2 \mathcal{L}^{-1}\left\{\frac{s-1}{(s-1)^{2}+3}\right\}-\frac{2}{\sqrt{3}} \mathcal{L}^{-1}\left\{\frac{\sqrt{3}}{(s-1)^{2}+3}\right\} \\
&=2 e^{t} \cos \sqrt{3} t-\frac{2}{\sqrt{3}} e^{t} \sin \sqrt{3} t
\end{aligned}

** Problem 19

*** Statement
    \begin{equation*}
y^{\prime \prime}+y=\left\{\begin{array}{ll}
t, & 0 \leq t<1 \\
2-t, & 1 \leq t<2, \\
0, & 2 \leq t<\infty
\end{array} \quad y(0)=0, \quad y^{\prime}(0)=0\right.
\end{equation*}

*** Solution
    Let $f(t)$ represent the piecewise function on the right side.
$$
y^{\prime \prime}+y=f(t)=\left\{\begin{array}{ll}
t, & 0 \leq t<1 \\
2-t, & 1 \leq t<2 \\
0, & 2 \leq t<\infty
\end{array}\right.
$$
Because this ODE is linear, the Laplace transform can be applied to solve it. The Laplace transform of a function $y(t)$ is defined here as
$$
Y(s)=\mathcal{L}\{y(t)\}=\int_{0}^{\infty} e^{-s t} y(t) d t .
$$
Consequently, the first and second derivatives transform as follows.

\begin{aligned}
\mathcal{L}\left\{\frac{d y}{d t}\right\} &=s Y(s)-y(0) \\
\mathcal{L}\left\{\frac{d^{2} y}{d t^{2}}\right\} &=s^{2} Y(s)-s y(0)-y^{\prime}(0)
\end{aligned}

Apply the Laplace transform to both sides of the ODE.

$$
\mathcal{L}\left\{y^{\prime \prime}+y\right\}=\mathcal{L}\{f(t)\}
$$

Use the fact that the transform is a linear operator.

\begin{array}{c}
\mathcal{L}\left\{y^{\prime \prime}\right\}+\mathcal{L}\{y\}=\mathcal{L}\{f(t)\} \\
{\left[s^{2} Y(s)-s y(0)-y^{\prime}(0)\right]+Y(s)=\int_{0}^{\infty} e^{-s t} f(t) d t}
\end{array}

Plug in the initial conditions, $y(0)=0$ and $y^{\prime}(0)=0$, and $f(t)$.

\begin{aligned}
\left[s^{2} Y(s)\right] &+Y(s)=\int_{0}^{1} e^{-s t}(t) d t+\int_{1}^{2} e^{-s t}(2-t) d t+\int_{2}^{\infty} e^{-s t}(0) d t \\
\left(s^{2}+1\right) Y(s) &=\int_{0}^{1} t e^{-s t} d t+2 \int_{1}^{2} e^{-s t} d t-\int_{1}^{2} t e^{-s t} d t \\
&=\frac{1-(s+1) e^{-s}}{s^{2}}+2 \frac{e^{-s}-e^{-2 s}}{s}-\frac{-e^{-2 s}-2 s e^{-2 s}+(s+1) e^{-s}}{s^{2}} \\
&=\frac{1}{s^{2}}+\frac{e^{-2 s}}{s^{2}}-\frac{2 e^{-s}}{s^{2}}
\end{aligned}

Divide both sides by $s^{2}+1$.

\begin{aligned}
Y(s) &=\frac{1}{s^{2}\left(s^{2}+1\right)}+\frac{e^{-2 s}}{s^{2}\left(s^{2}+1\right)}-\frac{2 e^{-s}}{s^{2}\left(s^{2}+1\right)} \\
&=\frac{1}{s^{2}}-\frac{1}{s^{2}+1}+\left(\frac{1}{s^{2}}-\frac{1}{s^{2}+1}\right) e^{-2 s}-2\left(\frac{1}{s^{2}}-\frac{1}{s^{2}+1}\right) e^{-s}
\end{aligned}

Take the inverse Laplace transform of $Y(s)$ now to recover $y(t)$. Note that $H(t)$ is the Heaviside function, which is defined to be 1 if $t>0$ and 0 if $t<0$.

\begin{aligned}
y(t) &=\mathcal{L}^{-1}\{Y(s)\} \\
&=\mathcal{L}^{-1}\left\{\frac{1}{s^{2}}-\frac{1}{s^{2}+1}+\left(\frac{1}{s^{2}}-\frac{1}{s^{2}+1}\right) e^{-2 s}-2\left(\frac{1}{s^{2}}-\frac{1}{s^{2}+1}\right) e^{-s}\right\} \\
&=\mathcal{L}^{-1}\left\{\frac{1}{s^{2}}-\frac{1}{s^{2}+1}\right\}+\mathcal{L}^{-1}\left\{\left(\frac{1}{s^{2}}-\frac{1}{s^{2}+1}\right) e^{-2 s}\right\}-2 \mathcal{L}^{-1}\left\{\left(\frac{1}{s^{2}}-\frac{1}{s^{2}+1}\right) e^{-s}\right\} \\
&=(t-\sin t)+[(t-2)-\sin (t-2)] H(t-2)-2[(t-1)-\sin (t-1)] H(t-1)
\end{aligned}

** Problem 22
   
*** Statement
    \begin{equation}
f(t)=t e^{a t}
\end{equation}

*** Solution
    The Laplace transform of a function $f(t)$ is defined here as
$$
F(s)=\mathcal{L}\{f(t)\}=\int_{0}^{\infty} e^{-s t} f(t) d t
$$

    Substitute the given function and evaluate the integral.

\begin{aligned}
F(s) &=\int_{0}^{\infty} e^{-s t} t e^{a t} d t \\
&=\int_{0}^{\infty}\left(-\frac{\partial}{\partial s} e^{-s t}\right) e^{a t} d t \\
&=-\frac{d}{d s} \int_{0}^{\infty} e^{-s t} e^{a t} d t \\
&=-\frac{d}{d s} \int_{0}^{\infty} e^{(a-s) t} d t \\
&=-\frac{d}{d s}\left[\left.\frac{1}{a-s} e^{(a-s) t}\right|_{0} ^{\infty}\right] \\
&=-\frac{d}{d s}\left(\frac{1}{s-a}\right) \\
&=-\left[-\frac{1}{(s-a)^{2}}\right] \\
&=\frac{1}{(s-a)^{2}}
\end{aligned}

* Section 6.3
  
** Problem 7

*** Statement
    \begin{equation*}
 f(t)=\left\{\begin{array}{ll}
 1, & 0 \leq t<2 \\
 e^{-(t-2)}, & t \geq 2
 \end{array}\right.
 \end{equation*}

*** Solution
    Write $f(t)$ in terms of the Heaviside function, $H(t)$, which is defined to be 1 if $t>0$ and 0 if $t<0$.

\begin{aligned}
f(t) &=1[H(t)-H(t-2)]+e^{-(t-2)} H(t-2) \\
&=H(t)+\left[e^{-(t-2)}-1\right] H(t-2) \\
&=u_{0}(t)+\left[e^{-(t-2)}-1\right] u_{2}(t)
\end{aligned}

** Problem 13
   
*** Statement
    \begin{equation*}
F(s)=\frac{3 !}{(s-2)^{4}}
\end{equation*}

*** Solution
    Apply the two transforms,
$$
\mathcal{L}\left\{t^{n}\right\}=\frac{n !}{s^{n+1}} \quad \text { and } \quad \mathcal{L}\left\{e^{c t} f(t)\right\}=F(s-c),
$$
together to solve this problem.

\begin{aligned}
f(t) &=\mathcal{L}^{-1}\{F(s)\} \\
&=\mathcal{L}^{-1}\left\{\frac{3 !}{(s-2)^{4}}\right\} \\
&=t^{3} e^{2 t}
\end{aligned}

** Problem 16
   
*** Statement
    \begin{equation*}
F(s)=\frac{e^{-s}+e^{-2 s}-e^{-3 s}-e^{-4 s}}{s}
\end{equation*}

*** Solution
    Apply the two transforms,
$$
\mathcal{L}\left\{t^{n}\right\}=\frac{n !}{s^{n+1}} \quad \text { and } \quad \mathcal{L}\{f(t-c) H(t-c)\}=F(s) e^{-c s}
$$
together to solve this problem.

\begin{aligned}
f(t) &=\mathcal{L}^{-1}\{F(s)\} \\
&=\mathcal{L}^{-1}\left\{\frac{e^{-s}+e^{-2 s}-e^{-3 s}-e^{-4 s}}{s}\right\} \\
&=\mathcal{L}^{-1}\left\{\frac{1}{s} e^{-s}\right\}+\mathcal{L}^{-1}\left\{\frac{1}{s} e^{-2 s}\right\}-\mathcal{L}^{-1}\left\{\frac{1}{s} e^{-3 s}\right\}-\mathcal{L}^{-1}\left\{\frac{1}{s} e^{-4 s}\right\} \\
&=(t-1)^{0} H(t-1)+(t-2)^{0} H(t-2)-(t-3)^{0} H(t-3)-(t-4)^{0} H(t-4) \\
&=H(t-1)+H(t-2)-H(t-3)-H(t-4) \\
&=u_{1}(t)+u_{2}(t)-u_{3}(t)-u_{4}(t)
\end{aligned}

** Problem 20
   
*** Statement
    \begin{equation*}
F(s)=\frac{1}{9 s^{2}-12 s+3}
\end{equation*}

*** Solution
    Observe that the denominator can be written in terms of $3 s$.
$$
F(s)=\frac{1}{(3 s)^{2}-4(3 s)+3}
$$
Factor the denominator.
$$
F(s)=\frac{1}{[(3 s)-1][(3 s)-3]}
$$
Partially decompose the fraction.
$$
F(s)=\frac{-\frac{1}{2}}{(3 s)-1}+\frac{\frac{1}{2}}{(3 s)-3}
$$
Apply the two transforms,
$$
\mathcal{L}\left\{e^{a t}\right\}=\frac{1}{s-a} \quad \text { and } \quad F(k s)=\mathcal{L}\left\{\frac{1}{k} f\left(\frac{t}{k}\right)\right\},
$$
together to get $f(t)$

\begin{aligned}
f(t) &=\mathcal{L}^{-1}\{F(s)\} \\
&=-\frac{1}{2}\left(\frac{1}{3} e^{t / 3}\right)+\frac{1}{2}\left(\frac{1}{3} e^{3 t / 3}\right) \\
&=-\frac{1}{6} e^{t / 3}+\frac{1}{6} e^{t} \\
&=\frac{1}{6}\left(e^{t}-e^{t / 3}\right)
\end{aligned}

* Section 6.4
  
** Problem 1

*** Statement
    \begin{equation*}
y^{\prime \prime}+y=f(t) ; \quad y(0)=0, \quad y^{\prime}(0)=1 ; \quad f(t)=\left\{\begin{array}{ll}
1, & 0 \leq t<3 \pi \\
0, & 3 \pi \leq t<\infty
\end{array}\right.
\end{equation*}

*** Solution
    Because the ODE is linear, the Laplace transform can be applied to solve it. The Laplace transform of a function $y(t)$ is defined here as
$$
Y(s)=\mathcal{L}\{y(t)\}=\int_{0}^{\infty} e^{-s t} y(t) d t
$$
Consequently, the first and second derivatives transform as follows.
Apply the Laplace transform to both sides of the ODE.
$$
\mathcal{L}\left\{y^{\prime \prime}+y\right\}=\mathcal{L}\{f(t)\}
$$
Use the fact that the transform is a linear operator.

\begin{array}{c}
\mathcal{L}\left\{y^{\prime \prime}\right\}+\mathcal{L}\{y\}=\mathcal{L}\{f(t)\} \\
{\left[s^{2} Y(s)-s y(0)-y^{\prime}(0)\right]+Y(s)=\int_{0}^{3 \pi} e^{-s t}(1) d t+\int_{3 \pi}^{\infty} e^{-s t}(0) d t}
\end{array}

Plug in the initial conditions, $y(0)=0$ and $y^{\prime}(0)=1$.
$$
\left[s^{2} Y(s)-1\right]+Y(s)=\int_{0}^{3 \pi} e^{-s t} d t
$$

As a result of applying the Laplace transform, the ODE has reduced to an algebraic equation for $Y$, the transformed solution.

\begin{array}{c}
\left(s^{2}+1\right) Y(s)-1=\left.\left(-\frac{1}{s} e^{-s t}\right)\right|_{0} ^{3 \pi} \\
\left(s^{2}+1\right) Y(s)=\frac{1}{s}-\frac{1}{s} e^{-3 \pi s}+1 \\
Y(s)=\frac{1}{s\left(s^{2}+1\right)}-\frac{1}{s\left(s^{2}+1\right)} e^{-3 \pi s}+\frac{1}{s^{2}+1} \\
=\left(\frac{1}{s}-\frac{s}{s^{2}+1}\right)-\left(\frac{1}{s}-\frac{s}{s^{2}+1}\right) e^{-3 \pi s}+\frac{1}{s^{2}+1}
\end{array}

Take the inverse Laplace transform of $Y(s)$ now to get $y(t)$.

\begin{aligned}
y(t) &=\mathcal{L}^{-1}\{Y(s)\} \\
&=\mathcal{L}^{-1}\left\{\left(\frac{1}{s}-\frac{s}{s^{2}+1}\right)-\left(\frac{1}{s}-\frac{s}{s^{2}+1}\right) e^{-3 \pi s}+\frac{1}{s^{2}+1}\right\} \\
&=(1-\cos t)-[1-\cos (t-3 \pi)] H(t-3 \pi)+\sin t \\
&=1+\sin t-\cos t-[1-\cos (t-\pi)] H(t-3 \pi) \\
&=1+\sin t-\cos t-(1+\cos t) H(t-3 \pi) \\
&=1+\sin t-\cos t-(1+\cos t) u_{3 \pi}(t)
\end{aligned}



** Problem 2

*** Solution

  Evaluate the inverse Laplace transforms.

In order to write $Y(s)$ in terms of known transforms, use partial fraction decomposition.
$$
\frac{1}{s\left(s^{2}+2 s+2\right)}=\frac{A}{s}+\frac{B s+C}{s^{2}+2 s+2}
$$
Multiply both sides by $s\left(s^{2}+2 s+2\right)$.
$$
1=A\left(s^{2}+2 s+2\right)+(B s+C) s
$$
Plug in three random values of $s$ to get a system of three equations for $A, B$, and $C .$

\begin{array}{ll}
s=0: & 1=2 A \\
s=1: & 1=5 A+B+C \\
s=2: & 1=10 A+4 B+2 C
\end{array}

Solving this system yields $A=1 / 2, B=-1 / 2$, and $C=-1$.
$$
Y(s)=\left(\frac{1 / 2}{s}+\frac{-\frac{1}{2} s-1}{s^{2}+2 s+2}\right) e^{-\pi s}-\left(\frac{1 / 2}{s}+\frac{-\frac{1}{2} s-1}{s^{2}+2 s+2}\right) e^{-2 \pi s}+\frac{1}{s^{2}+2 s+2}
$$
Complete the square in the denominators.

\begin{aligned}
Y(s) &=\left(\frac{1 / 2}{s}+\frac{-\frac{1}{2} s-1}{s^{2}+2 s+1+2-1}\right) e^{-\pi s}-\left(\frac{1 / 2}{s}+\frac{-\frac{1}{2} s-1}{s^{2}+2 s+1+2-1}\right) e^{-2 \pi s}+\frac{1}{s^{2}+2 s+1+2-1} \\
&=\left[\frac{1 / 2}{s}+\frac{-\frac{1}{2} s-1}{(s+1)^{2}+1}\right] e^{-\pi s}-\left[\frac{1 / 2}{s}+\frac{-\frac{1}{2} s-1}{(s+1)^{2}+1}\right] e^{-2 \pi s}+\frac{1}{(s+1)^{2}+1}
\end{aligned}

Make it so that $s+1$ appears in the numerators.

\begin{aligned}
Y(s)=&\left[\frac{1 / 2}{s}+\frac{-\frac{1}{2}(s+1)-\frac{1}{2}}{(s+1)^{2}+1}\right] e^{-\pi s}-\left[\frac{1 / 2}{s}+\frac{-\frac{1}{2}(s+1)-\frac{1}{2}}{(s+1)^{2}+1}\right] e^{-2 \pi s}+\frac{1}{(s+1)^{2}+1} \\
=&\left[\frac{1 / 2}{s}-\frac{1}{2} \frac{s+1}{(s+1)^{2}+1}-\frac{1}{2} \frac{1}{(s+1)^{2}+1}\right] e^{-\pi s} \\
&-\left[\frac{1 / 2}{s}-\frac{1}{2} \frac{s+1}{(s+1)^{2}+1}-\frac{1}{2} \frac{1}{(s+1)^{2}+1}\right] e^{-2 \pi s}+\frac{1}{(s+1)^{2}+1}
\end{aligned}

Take the inverse Laplace transform of $Y(s)$ now to get $y(t)$.
$$
y(t)=\mathcal{L}^{-1}\{Y(s)\}
$$


\begin{aligned}
=\mathcal{L}^{-1}\left\{\left[\frac{1 / 2}{s}\right.\right.&\left.-\frac{1}{2} \frac{s+1}{(s+1)^{2}+1}-\frac{1}{2} \frac{1}{(s+1)^{2}+1}\right] e^{-\pi s} \\
&\left.-\left[\frac{1 / 2}{s}-\frac{1}{2} \frac{s+1}{(s+1)^{2}+1}-\frac{1}{2} \frac{1}{(s+1)^{2}+1}\right] e^{-2 \pi s}+\frac{1}{(s+1)^{2}+1}\right\} \\
=\mathcal{L}^{-1}\left\{\left[\frac{1 / 2}{s}-\right.\right.&\left.\left.\frac{1}{2} \frac{s+1}{(s+1)^{2}+1}-\frac{1}{2} \frac{1}{(s+1)^{2}+1}\right] e^{-\pi s}\right\} \\
&-\mathcal{L}^{-1}\left\{\left[\frac{1 / 2}{s}-\frac{1}{2} \frac{s+1}{(s+1)^{2}+1}-\frac{1}{2} \frac{1}{(s+1)^{2}+1}\right] e^{-2 \pi s}\right\}+\mathcal{L}^{-1}\left\{\frac{1}{(s+1)^{2}+1}\right\}
\end{aligned}
  
\begin{aligned}
y(t)=&\left[\frac{1}{2}-\frac{1}{2} e^{-(t-\pi)} \cos (t-\pi)-\frac{1}{2} e^{-(t-\pi)} \sin (t-\pi)\right] H(t-\pi) \\
-\left[\frac{1}{2}-\frac{1}{2} e^{-(t-2 \pi)} \cos (t-2 \pi)-\frac{1}{2} e^{-(t-2 \pi)} \sin (t-2 \pi)\right] H(t-2 \pi)+e^{-t} \sin t \\
=&\left(\frac{1}{2}+\frac{1}{2} e^{\pi-t} \cos t+\frac{1}{2} e^{\pi-t} \sin t\right) H(t-\pi) \\
\quad-\left(\frac{1}{2}-\frac{1}{2} e^{2 \pi-t} \cos t-\frac{1}{2} e^{2 \pi-t} \sin t\right) H(t-2 \pi)+e^{-t} \sin t \\
=\frac{1}{2}\left(1+e^{\pi-t} \cos t+e^{\pi-t} \sin t\right) H(t-\pi) \\
-\frac{1}{2}\left(1-e^{2 \pi-t} \cos t-e^{2 \pi-t} \sin t\right) H(t-2 \pi)+e^{-t} \sin t
\end{aligned}

Therefore,
$$
y(t)=\frac{1}{2}\left(1+e^{\pi-t} \cos t+e^{\pi-t} \sin t\right) u_{\pi}(t)-\frac{1}{2}\left(1-e^{2 \pi-t} \cos t-e^{2 \pi-t} \sin t\right) u_{2 \pi}(t)+e^{-t} \sin t
$$  
